verifier/template/lean/Project.lean
@@ -1,4 +1,0 @@
-import Project.IsEven.Proof
-import Project.IsEven.Run
-import Project.IsOdd.Proof
-import Project.IsOdd.Run
